template-coq/theories/Substitution.v
@@ -1,0 +1,1093 @@
+(* Distributed under the terms of the MIT license.   *)
+
+From Coq Require Import Bool String List Program BinPos Compare_dec Omega Lia.
+From Template Require Import config utils Ast AstUtils Induction utils LiftSubst Typing.
+From Template Require Import WeakeningEnv Closed.
+
+(** * Substitution lemmas for typing derivations. *)
+
+Set Asymmetric Patterns.
+
+Generalizable Variables Σ Γ t T.
+
+Definition subst_decl s k (d : context_decl) := map_decl (subst s k) d.
+
+Definition subst_context n k (Γ : context) : context :=
+  List.rev (mapi (fun k' decl => subst_decl n (k + k') decl) (List.rev Γ)).
+
+Definition wf_decl_pred : global_context -> context -> term -> term -> Type :=
+  (fun _ _ t T => Ast.wf t /\ Ast.wf T).
+
+Lemma subst_decl0 Σ Γ k d : on_local_decl wf_decl_pred Σ Γ d -> subst_decl [] k d = d.
+Proof.
+  unfold wf_decl_pred; intros Hd; destruct d; destruct decl_body;
+    unfold on_local_decl in Hd; unfold subst_decl, map_decl; simpl in *;
+    f_equal; simpl; rewrite subst_empty; intuition trivial.
+  destruct Hd as [u Hu]; intuition trivial.
+Qed.
+
+Definition on_some {A} (P : A -> Type) (o : option A) :=
+  match o with
+  | Some t => P t
+  | None => False
+  end.
+
+Lemma nth_error_All_local_env `{checker_flags} {P Σ Γ n} (isdecl : n < #|Γ|) :
+  All_local_env P Σ Γ ->
+  on_some (on_local_decl P Σ (skipn (S n) Γ)) (nth_error Γ n).
+Proof.
+  induction 1 in n, isdecl |- *. red; simpl.
+  - destruct n; simpl; inv isdecl.
+  - destruct n. red; simpl. now exists u.
+    simpl. apply IHX. simpl in isdecl. lia.
+  - destruct n. auto.
+    apply IHX. simpl in *. lia.
+Qed.
+
+Lemma All_local_env_wf_decl_inv:
+  forall (H : checker_flags) (Σ : global_context) (a : context_decl) (Γ : list context_decl)
+         (X : All_local_env wf_decl_pred Σ (a :: Γ)),
+    on_local_decl wf_decl_pred Σ Γ a * All_local_env wf_decl_pred Σ Γ.
+Proof.
+  intros H Σ a Γ X.
+  inv X; intuition; red; simpl; eauto.
+Qed.
+
+Lemma subst0_context `{checker_flags} Σ k Γ : All_local_env wf_decl_pred Σ Γ -> subst_context [] k Γ = Γ.
+Proof.
+  unfold subst_context.
+  rewrite rev_mapi. rewrite List.rev_involutive.
+  unfold mapi. generalize 0. generalize #|List.rev Γ|.
+  induction Γ; intros; simpl; trivial.
+  eapply All_local_env_wf_decl_inv in X as [Ha HΓ].
+  erewrite subst_decl0; f_equal; eauto.
+Qed.
+
+Lemma subst_context_length s k Γ : #|subst_context s k Γ| = #|Γ|.
+Proof.
+  unfold subst_context. now rewrite !List.rev_length, mapi_length, List.rev_length.
+Qed.
+Hint Rewrite subst_context_length : subst.
+
+
+Lemma subst_context_snoc0 s k Γ d : subst_context s k (d :: Γ) = subst_context s k Γ ,, subst_decl s (#|Γ| + k) d.
+Proof.
+  unfold subst_context.
+  rewrite !rev_mapi, !rev_involutive. unfold mapi; rewrite mapi_rec_eqn.
+  unfold snoc. f_equal. now rewrite Nat.sub_0_r, Nat.add_comm, List.rev_length.
+  rewrite mapi_rec_Sk. simpl. apply mapi_rec_ext. intros.
+  rewrite app_length, !List.rev_length. simpl. f_equal. lia.
+Qed.
+Hint Rewrite subst_context_snoc0 : subst.
+
+Lemma subst_context_snoc s k Γ d : subst_context s k (Γ ,, d) = subst_context s k Γ ,, subst_decl s (#|Γ| + k) d.
+Proof.
+  unfold snoc. apply subst_context_snoc0.
+Qed.
+Hint Rewrite subst_context_snoc : subst.
+
+Lemma subst_context_alt s k Γ :
+  subst_context s k Γ =
+  mapi (fun k' d => subst_decl s (pred #|Γ| - k' + k) d) Γ.
+Proof.
+  unfold subst_context. rewrite rev_mapi. rewrite List.rev_involutive.
+  apply mapi_ext. intros. f_equal. now rewrite List.rev_length.
+Qed.
+
+Lemma subst_context_app s k Γ Δ :
+  subst_context s k (Γ ,,, Δ) = subst_context s k Γ ,,, subst_context s (#|Γ| + k) Δ.
+Proof.
+  unfold subst_context, app_context.
+  rewrite List.rev_app_distr.
+  rewrite mapi_app. rewrite <- List.rev_app_distr. f_equal. f_equal.
+  apply mapi_ext. intros. f_equal. rewrite List.rev_length. lia.
+Qed.
+
+Lemma nth_error_subst_context (Γ' : context) s (v : nat) k :
+    nth_error (subst_context s k Γ') v =
+    option_map (subst_decl s (#|Γ'| - S v + k)) (nth_error Γ' v).
+Proof.
+  induction Γ' in v |- *; intros.
+  - simpl. unfold subst_context; simpl; rewrite nth_error_nil. easy.
+  - simpl. destruct v; rewrite subst_context_snoc0.
+    + simpl. repeat f_equal; try lia.
+    + simpl. rewrite IHΓ'; simpl in *; (lia || congruence).
+Qed.
+
+Inductive subs `{cf : checker_flags} Σ (Γ : context) : list term -> context -> Type :=
+| emptys : subs Σ Γ [] []
+| cons_ass Δ s na t T : subs Σ Γ s Δ ->
+              Σ ;;; Γ |- t : substl s T ->
+                             subs Σ Γ (t :: s) (Δ ,, vass na T).
+(* | cons_let Δ s na t T : subs Σ Γ s Δ -> *)
+(*               Σ ;;; Γ |- substl s t : substl s T -> *)
+(*               subs Σ Γ (substl s t :: s) (Δ ,, vdef na t T). *)
+
+Lemma subst_length `{checker_flags} Σ Γ s Γ' : subs Σ Γ s Γ' -> #|s| = #|Γ'|.
+Proof.
+  induction 1; simpl; auto with arith.
+Qed.
+
+Hint Rewrite @app_context_length @subst_context_length : wf.
+
+Lemma subs_nth_error_ge `{checker_flags} Σ Γ Γ' Γ'' v s :
+  subs Σ Γ s Γ' ->
+  #|Γ' ,,, Γ''| <= v ->
+  nth_error (Γ ,,, Γ' ,,, Γ'') v =
+  nth_error (Γ ,,, subst_context s 0 Γ'') (v - #|Γ'|).
+Proof.
+  simpl.
+  intros. rewrite app_context_length in H0.
+  rewrite !nth_error_app_ge; autorewrite with wf; f_equal; try lia.
+Qed.
+
+Lemma subs_nth_error_lt `{checker_flags} Σ Γ Γ' Γ'' v s :
+  subs Σ Γ s Γ' ->
+  v < #|Γ''| ->
+  nth_error (Γ ,,, subst_context s 0 Γ'') v =
+  option_map (map_decl (subst s (#|Γ''| - S v))) (nth_error (Γ ,,, Γ' ,,, Γ'') v).
+Proof.
+  simpl. intros Hs Hv.
+  rewrite !nth_error_app_lt; autorewrite with wf; f_equal; try lia.
+  erewrite nth_error_subst_context. f_equal. unfold subst_decl. rewrite Nat.add_0_r. reflexivity.
+Qed.
+
+Lemma subst_iota_red s k pars c args brs :
+  subst s k (iota_red pars c args brs) =
+  iota_red pars c (List.map (subst s k) args) (List.map (on_snd (subst s k)) brs).
+Proof.
+  unfold iota_red. rewrite !subst_mkApps. f_equal; auto using map_skipn.
+  rewrite nth_map; simpl; auto.
+Qed.
+
+Lemma fix_subst_length mfix : #|fix_subst mfix| = #|mfix|.
+Proof.
+  unfold fix_subst. generalize (tFix mfix). intros.
+  induction mfix; simpl; auto.
+Qed.
+
+Lemma cofix_subst_length mfix : #|cofix_subst mfix| = #|mfix|.
+Proof.
+  unfold cofix_subst. generalize (tCoFix mfix). intros.
+  induction mfix; simpl; auto.
+Qed.
+Hint Rewrite fix_subst_length cofix_subst_length : wf.
+
+Lemma subst_unfold_fix n k mfix idx narg fn :
+  Forall Ast.wf n ->
+  unfold_fix mfix idx = Some (narg, fn) ->
+  unfold_fix (map (map_def (subst n k) (subst n (#|mfix| + k))) mfix) idx = Some (narg, subst n k fn).
+Proof.
+  unfold unfold_fix. intros wfn.
+  rewrite nth_error_map. destruct (nth_error mfix idx) eqn:Hdef; try congruence.
+  intros [= <- <-]. simpl. repeat f_equal. unfold substl.
+  erewrite (distr_subst_rec _ _ _ wfn k 0).
+  rewrite fix_subst_length. simpl. f_equal.
+  unfold fix_subst. rewrite !map_length.
+  generalize #|mfix| at 2 3. induction n0; auto. simpl.
+  f_equal. apply IHn0.
+Qed.
+Hint Resolve subst_unfold_fix.
+
+Lemma subst_unfold_cofix n k mfix idx narg fn :
+  Forall Ast.wf n ->
+  unfold_cofix mfix idx = Some (narg, fn) ->
+  unfold_cofix (map (map_def (subst n k) (subst n (#|mfix| + k))) mfix) idx = Some (narg, subst n k fn).
+Proof.
+  unfold unfold_cofix. intros wfn.
+  rewrite nth_error_map. destruct (nth_error mfix idx) eqn:Hdef; try congruence.
+  intros [= <- <-]. simpl. repeat f_equal. unfold substl.
+  erewrite (distr_subst_rec _ _ _ wfn k 0).
+  rewrite cofix_subst_length. simpl. f_equal.
+  unfold cofix_subst. rewrite !map_length.
+  generalize #|mfix| at 2 3. induction n0; auto. simpl.
+  f_equal. apply IHn0.
+Qed.
+Hint Resolve subst_unfold_cofix.
+
+Lemma subst_is_constructor:
+  forall (args : list term) (narg : nat) n k,
+    is_constructor narg args = true -> is_constructor narg (map (subst n k) args) = true.
+Proof.
+  intros args narg.
+  unfold is_constructor; intros.
+  rewrite nth_error_map. destruct nth_error; try discriminate. simpl. intros.
+  destruct t; try discriminate || reflexivity.
+  destruct t; try discriminate || reflexivity. simpl.
+  destruct l; auto.
+Qed.
+Hint Resolve subst_is_constructor.
+Hint Constructors All_local_env.
+
+Lemma typed_subst `{checker_flags} Σ Γ t T n k :
+  wf Σ -> wf_local Σ Γ -> k >= #|Γ| ->
+  Σ ;;; Γ |- t : T -> subst n k t = t.
+Proof.
+  intros wfΣ wfΓ Hk Hty.
+  pose proof (typing_wf _ wfΣ _ wfΓ _ _ Hty) as [wft wfT].
+  apply typecheck_closed in Hty; eauto.
+  destruct Hty as [_ Hcl].
+  rewrite andb_true_iff in Hcl. destruct Hcl as [clb clty].
+  pose proof (closed_upwards _ _ clb k).
+  simpl in *. forward H0 by lia.
+  apply (subst_closedn n) in H0; auto.
+Qed.
+
+Definition option_default {A B} (f : A -> B) (o : option A) (b : B) :=
+  match o with Some x => f x | None => b end.
+
+Lemma declared_decl_closed `{checker_flags} Σ cst decl :
+  wf Σ ->
+  lookup_env (fst Σ) cst = Some decl ->
+  on_global_decl (fun Σ Γ b t =>
+                    match b with Some b => Ast.wf b | None => True end /\ Ast.wf t /\
+                    option_default (closedn #|Γ|) b true && closedn #|Γ| t = true) Σ decl.
+Proof.
+  intros.
+  eapply weaken_lookup_on_global_env; try red; eauto.
+  eapply on_global_decls_impl; cycle 1.
+  eapply on_global_decls_mix.
+  apply (env_prop_sigma _ typecheck_closed _ X).
+  apply (env_prop_sigma _ typing_wf_gen _ X).
+  intros.
+  simpl in X1. destruct X1 as [Hcl Hwf]. red in Hcl, Hwf.
+  destruct t; simpl; intuition auto.
+  destruct Hwf; simpl; intuition auto.
+  destruct Hwf; simpl; intuition auto.
+  destruct Hcl; simpl; intuition auto.
+  rewrite andb_true_iff in e. intuition.
+Qed.
+
+Lemma subst_declared_constant `{checker_flags} Σ cst decl n k :
+  wf Σ ->
+  declared_constant (fst Σ) cst decl ->
+  map_constant_body (subst n k) decl = decl.
+Proof.
+  intros.
+  eapply declared_decl_closed in H0; eauto.
+  unfold map_constant_body.
+  do 2 red in H0. destruct decl as [ty [body|] univs]; simpl in *.
+  rewrite andb_true_iff in H0. intuition.
+  f_equal. apply (subst_closedn n k) in H0; eauto using closed_upwards with arith.
+  f_equal. apply (subst_closedn n k) in H1; eauto using closed_upwards with arith.
+  red in H0. f_equal.
+  intuition. simpl in H3.
+  eapply subst_closedn; eauto using closed_upwards with arith.
+Qed.
+
+Definition subst_mutual_inductive_body n k mind m :=
+  map_mutual_inductive_body mind (fun Γ => subst n (#|Γ| + k)) m.
+
+Lemma subst_declared_minductive `{checker_flags} Σ cst decl n k :
+  wf Σ ->
+  declared_minductive (fst Σ) cst decl ->
+  subst_mutual_inductive_body n k cst decl = decl.
+Proof.
+  unfold declared_minductive.
+  intros.
+  eapply lookup_on_global_env in H0; eauto.
+  destruct H0 as [Σ' [wfΣ' decl']].
+  do 2 red in decl'.
+  destruct decl. simpl in *. f_equal.
+  revert decl'. generalize ind_bodies at 2 4 5.
+  intros.
+  eapply Alli_map_id in decl'. eauto.
+  clear decl'. intros.
+  destruct x; simpl in *.
+  destruct (decompose_prod_assum [] ind_type) eqn:Heq.
+  destruct (decompose_prod_assum [] (subst n k ind_type)) eqn:Heq'.
+  destruct X0. simpl in *.
+  assert (subst n k ind_type = ind_type).
+  destruct onArity as [s Hs].
+  eapply typed_subst; eauto. simpl; lia.
+  rewrite H0 in Heq'. rewrite Heq in Heq'. revert Heq'; intros [= <- <-].
+  f_equal; auto.
+  apply (All_map_id onConstructors).
+  intros [[x p] n']. intros [s Hty].
+  unfold on_pi2; f_equal; f_equal. eapply typed_subst. 4:eapply Hty. wf. wf. lia.
+  rewrite Heq in onProjections. destruct onProjections as [_ onProjections].
+  apply (All_map_id onProjections).
+  intros [x p]. intros [s Hty].
+  unfold on_snd; f_equal; f_equal.
+  eapply typed_subst. 4:eapply Hty. wf. wf. simpl. lia.
+Qed.
+
+Lemma subst_declared_inductive `{checker_flags} Σ ind mdecl idecl n k :
+  wf Σ ->
+  declared_inductive (fst Σ) ind mdecl idecl ->
+  map_one_inductive_body (inductive_mind ind) (polymorphic_instance (mdecl.(ind_universes))) (arities_context mdecl.(ind_bodies)) (fun Γ => subst n (#|Γ| + k)) (inductive_ind ind) idecl = idecl.
+Proof.
+  unfold declared_inductive. intros wfΣ [Hmdecl Hidecl].
+  destruct Σ. eapply (subst_declared_minductive _ _ _ n k) in Hmdecl.
+  unfold subst_mutual_inductive_body in Hmdecl.
+  destruct mdecl. simpl in *.
+  injection Hmdecl. intros Heq.
+  clear Hmdecl.
+  pose proof Hidecl as Hidecl'.
+  rewrite <- Heq in Hidecl'.
+  rewrite nth_error_mapi in Hidecl'.
+  clear Heq.
+  unfold option_map in Hidecl'. rewrite Hidecl in Hidecl'.
+  congruence. auto.
+Qed.
+
+Lemma substl_inds_subst ind u mdecl n k t :
+  Forall Ast.wf n ->
+  (substl (inds (inductive_mind ind) u (ind_bodies mdecl))
+          (subst n (#|arities_context (ind_bodies mdecl)| + k) t)) =
+  subst n k (substl (inds (inductive_mind ind) u (ind_bodies mdecl)) t).
+Proof.
+  unfold substl. intros wfn.
+  pose proof (distr_subst_rec t (inds (inductive_mind ind) u (ind_bodies mdecl)) n wfn k 0).
+  simpl in H. rewrite H.
+  unfold arities_context. rewrite rev_map_length, inds_length.
+  f_equal. generalize (ind_bodies mdecl).
+  clear. intros.
+  induction l; unfold inds; simpl; auto. f_equal. auto.
+Qed.
+
+Lemma subst_declared_constructor `{checker_flags} Σ c u mdecl idecl cdecl n k :
+  wf Σ -> Forall Ast.wf n ->
+  declared_constructor (fst Σ) mdecl idecl c cdecl ->
+  subst (map (UnivSubst.subst_instance_constr u) n) k (type_of_constructor mdecl cdecl c u) = (type_of_constructor mdecl cdecl c u).
+Proof.
+  unfold declared_constructor. destruct c as [i ci]. intros wfΣ wfn [Hidecl Hcdecl].
+  destruct Σ. eapply (subst_declared_inductive _ _ _ _ n k) in Hidecl; eauto.
+  unfold type_of_constructor. destruct cdecl as [[id t'] arity].
+  destruct idecl; simpl in *.
+  destruct (decompose_prod_assum [] _) eqn:Heq.
+  injection Hidecl.
+  intros.
+  pose Hcdecl as Hcdecl'.
+  rewrite <- H1 in Hcdecl'.
+  rewrite nth_error_map in Hcdecl'. rewrite Hcdecl in Hcdecl'.
+  simpl in Hcdecl'. injection Hcdecl'.
+  intros.
+  rewrite <- H3 at 2.
+  rewrite <- substl_inds_subst. f_equal.
+  now rewrite <- UnivSubst.subst_subst_instance_constr.
+  apply Forall_map. unfold compose. eapply Forall_impl; eauto.
+  intros. now apply wf_subst_instance_constr.
+Qed.
+
+Lemma subst_declared_projection `{checker_flags} Σ c mdecl idecl pdecl n k :
+  wf Σ -> Forall Ast.wf n ->
+  declared_projection (fst Σ) mdecl idecl c pdecl ->
+  on_snd (subst n (S (ind_npars mdecl + k))) pdecl = pdecl.
+Proof.
+  unfold declared_projection. destruct c as [[i k'] ci].
+  intros wfΣ wfn [Hidecl Hcdecl].
+  simpl in *.
+  pose proof Hidecl. destruct H0 as [Hmdecl Hidecl'].
+  eapply lookup_on_global_env in Hmdecl; eauto.
+  destruct Hmdecl as [Σ' [wfΣ' ongdecl]].
+  red in ongdecl. red in ongdecl.
+  eapply nth_error_alli in Hidecl'; eauto.
+  apply onProjections in Hidecl'.
+  destruct decompose_prod_assum eqn:Heq.
+  destruct Hidecl' as [Hpars _].
+  destruct Σ. eapply (subst_declared_inductive _ _ _ _ n k) in Hidecl; eauto.
+  destruct pdecl as [id t'].
+  destruct idecl; simpl in *.
+  destruct (decompose_prod_assum _ _) eqn:Heq'.
+  injection Hidecl.
+  intros.
+  rewrite <- H2 in Heq. rewrite Heq in Heq'. injection Heq'. intros <- <-.
+  forward Hpars. destruct ind_projs; destruct ci; discriminate.
+  rewrite Hpars in H0.
+  pose proof Hcdecl as Hcdecl'.
+  rewrite <- H0 in Hcdecl.
+  rewrite nth_error_map in Hcdecl; eauto.
+  rewrite Hcdecl' in Hcdecl. simpl in Hcdecl.
+  congruence.
+Qed.
+
+Lemma map_vass_map_def g l n k :
+  (mapi (fun i (d : def term) => vass (dname d) (lift0 i (dtype d)))
+        (map (map_def (subst n k) g) l)) =
+  (mapi (fun i d => map_decl (subst n (i + k)) d) (mapi (fun i (d : def term) => vass (dname d) (lift0 i (dtype d))) l)).
+Proof.
+  rewrite mapi_mapi, mapi_map. apply mapi_ext.
+  intros. unfold map_decl, vass; simpl; f_equal.
+  rewrite commut_lift_subst_rec. f_equal; lia. lia.
+Qed.
+
+Lemma subst_fix_context:
+  forall (mfix : list (def term)) n (k : nat),
+    fix_context (map (map_def (subst n k) (subst n (#|mfix| + k))) mfix) =
+    subst_context n k (fix_context mfix).
+Proof.
+  intros mfix n k. unfold fix_context.
+  rewrite map_vass_map_def, rev_mapi.
+  fold (fix_context mfix).
+  rewrite (subst_context_alt n k (fix_context mfix)).
+  unfold subst_decl. now rewrite mapi_length, fix_context_length.
+Qed.
+
+Lemma All_local_env_subst `{checker_flags} (P Q : global_context -> context -> term -> term -> Type) Σ c n k :
+  All_local_env Q Σ c ->
+  (forall Γ t T,
+      Q Σ Γ t T -> P Σ (subst_context n k Γ) (subst n (#|Γ| + k) t) (subst n (#|Γ| + k) T)) ->
+  All_local_env P Σ (subst_context n k c).
+Proof.
+  intros Hq Hf. induction Hq in |- *; try econstructor; eauto;
+                  simpl; rewrite subst_context_snoc; econstructor; eauto.
+  simpl. eapply (Hf _ _ (tSort u)). eauto.
+Qed.
+
+Lemma subst_destArity ctx t n k :
+  Ast.wf t ->
+  match destArity ctx t with
+  | Some (args, s) =>
+    destArity (subst_context n k ctx) (subst n (#|ctx| + k) t) = Some (subst_context n k args, s)
+  | None => True
+  end.
+Proof.
+  intros wf; revert ctx.
+  induction wf in n, k |- * using Template.Induction.term_wf_forall_list_ind; intros ctx; simpl; trivial.
+
+  - specialize (IHwf0 n k (ctx,, vass n0 t)). rewrite subst_context_snoc in IHwf0.
+    simpl in IHwf0. unfold subst_decl, map_decl in IHwf0. unfold vass in *. simpl in IHwf0.
+    destruct destArity. destruct p. simpl in *. auto. exact I.
+  - specialize (IHwf1 n k (ctx,, vdef n0 t t0)). rewrite subst_context_snoc in IHwf1.
+    unfold vdef, subst_decl, map_decl in *. simpl in *.
+    destruct destArity as [[args s]|]. apply IHwf1. exact I.
+Qed.
+
+(* Lemma subst_instantiate_params n k args t k' : *)
+(*   closedn k' t = true -> Forall Ast.wf n -> *)
+(*   option_map (subst n k) (instantiate_params args t) = *)
+(*   instantiate_params (map (subst n k) args) (subst n k t). *)
+(* Proof. *)
+(*   induction args in t, n, k |- *. reflexivity. *)
+(*   simpl. destruct t; try (simpl; congruence). *)
+(*   - simpl. rewrite Nat.ltb_lt. intros IH. *)
+(*     destruct (leb_spec_Set k n0). lia. reflexivity. *)
+(*   - intros. rewrite IHargs. f_equal. unfold subst1. *)
+(*     simpl. f_equal. simpl in H. *)
+(*     rewrite andb_true_iff in H. destruct H. *)
+(*     rewrite distr_subst; simpl. reflexivity. auto. simpl in H. *)
+(*     unfold subst1. simpl. *)
+(*     replace k with (k + 0) by lia. *)
+(*     (* eapply (closedn_subst _ _ 0). admit. simpl. *) *)
+(*     (* replace (k + 0 + 1) with (S k) by lia. *) *)
+(*     (* now rewrite andb_true_iff in H. auto. *) *)
+(* Admitted. *)
+(* (*   - rewrite IHargs; f_equal. apply distr_lift_subst. *) *)
+(* (* Qed. *) *)
+(* Hint Rewrite subst_instantiate_params : lift. *)
+
+Lemma subst_decompose_prod_assum_rec ctx t n k :
+  let (ctx', t') := decompose_prod_assum ctx t in
+  (subst_context n k ctx', subst n (length ctx' + k) t') =
+  decompose_prod_assum (subst_context n k ctx) (subst n (length ctx + k) t).
+Proof.
+  induction t in n, k, ctx |- *; simpl;
+    try rewrite Nat.sub_diag, Nat.add_0_r; try (eauto; congruence).
+  - destruct (Nat.leb (#|ctx| + k) n0).
+    destruct nth_error eqn:Heq.
+  (* - eapply IHt1. *)
+  (* - specialize (IHt2 (ctx ,, vass n0 t1) n k). *)
+  (*   destruct decompose_prod_assum. rewrite IHt2. simpl. *)
+  (*   rewrite lift_context_snoc. reflexivity. *)
+  (* - specialize (IHt3 (ctx ,, vdef n0 t1 t2) n k). *)
+  (*   destruct decompose_prod_assum. rewrite IHt3. simpl. *)
+  (*   rewrite lift_context_snoc. reflexivity. *)
+Admitted.
+
+Lemma subst_decompose_prod_assum t n k :
+  let (ctx', t') := decompose_prod_assum [] t in
+  (subst_context n k ctx', subst n (length ctx' + k) t') =
+  decompose_prod_assum [] (subst n k t).
+Proof. apply subst_decompose_prod_assum_rec. Qed.
+
+Lemma decompose_app_subst n k t f a :
+  closedn k t = true ->
+  decompose_app t = (f, a) -> decompose_app (subst n k t) = (subst n k f, map (subst n k) a).
+Proof.
+  (* destruct t; simpl; intros [= <- <-]; try reflexivity. *)
+  (* simpl. *)
+  (* now destruct (Nat.leb k n0). Qed. *)
+Admitted.
+
+Lemma subst_it_mkProd_or_LetIn n k ctx t :
+  subst n k (it_mkProd_or_LetIn ctx t) =
+  it_mkProd_or_LetIn (subst_context n k ctx) (subst n (length ctx + k) t).
+Proof.
+  induction ctx in n, k, t |- *; simpl; try congruence.
+  pose (subst_context_snoc n k ctx a). unfold snoc in e. rewrite e. clear e.
+  simpl. destruct decl_body. now rewrite IHctx.
+  pose (subst_context_snoc n k ctx a). simpl. now rewrite IHctx.
+Qed.
+
+Lemma to_extended_list_subst n k c :
+  to_extended_list (subst_context n k c) = to_extended_list c.
+Proof.
+  unfold to_extended_list. generalize 0. generalize (@nil term) at 1 2.
+  induction c in n, k |- *; simpl; intros. reflexivity.
+  rewrite subst_context_snoc0. unfold snoc. simpl.
+  destruct a. destruct decl_body. unfold subst_decl, map_decl. simpl.
+  now rewrite IHc. simpl. apply IHc.
+Qed.
+
+Lemma to_extended_list_map_subst:
+  forall n (k : nat) (c : context), to_extended_list c = map (subst n (#|c| + k)) (to_extended_list c).
+Proof.
+  intros n k c.
+  pose proof (to_extended_list_lift_above c).
+  symmetry. apply_spec. intros.
+  destruct H0. intuition. subst x. simpl.
+  destruct (leb_spec_Set (#|c| + k) x0). lia. reflexivity.
+Qed.
+
+Lemma subst_types_of_case ind mdecl idecl args u p pty indctx pctx ps btys n k :
+  let f ctx := subst n (#|ctx| + k) in
+  let f_ctx := subst_context n k in
+  Ast.wf pty -> Ast.wf (ind_type idecl) ->
+  types_of_case ind mdecl idecl args u p pty = Some (indctx, pctx, ps, btys) ->
+  types_of_case ind mdecl (map_one_inductive_body (inductive_mind ind) (polymorphic_instance mdecl.(ind_universes))
+                                                  (arities_context mdecl.(ind_bodies)) f (inductive_ind ind) idecl)
+                (map (f []) args) u (f [] p) (f [] pty) =
+  Some (f_ctx indctx, f_ctx pctx, ps, map (on_snd (f [])) btys).
+Proof.
+  simpl. intros wfpty wfdecl. simpl.
+  unfold types_of_case. simpl.
+  pose proof (subst_destArity [] (ind_type idecl) n k wfdecl); trivial. simpl in H.
+  unfold subst_context in H. simpl in H. rewrite ind_type_map. simpl.
+  destruct destArity as [[ctx s] | ]; try congruence. rewrite H. clear H.
+  pose proof (subst_destArity [] pty n k wfpty); trivial. simpl in H.
+  unfold subst_context in H. simpl in H.
+  destruct destArity as [[ctx' s'] | ]; try congruence.
+  rewrite H; clear H.
+  assert(forall brs,
+         build_branches_type ind mdecl idecl args u p = brs ->
+         (build_branches_type ind mdecl
+         (map_one_inductive_body (inductive_mind ind) (polymorphic_instance (ind_universes mdecl))
+            (arities_context (ind_bodies mdecl)) (fun ctx0 : list context_decl => subst n (#|ctx0| + k))
+            (inductive_ind ind) idecl) (map (subst n k) args) u (subst n k p)) =
+         map (option_map (on_snd (subst n k))) brs).
+  unfold build_branches_type. simpl. intros brs. intros <-.
+  rewrite ind_ctors_map.
+  rewrite mapi_map, map_mapi. f_equal. extensionality i. extensionality x.
+  destruct x as [[id t] arity]. simpl.
+  rewrite <- UnivSubst.subst_subst_instance_constr.
+  rewrite substl_inds_subst.
+(*   rewrite <- subst_instantiate_params. *)
+(*   destruct (instantiate_params _ _) eqn:Heqip. simpl. *)
+(*   epose proof (subst_decompose_prod_assum t0 n k). *)
+(*   destruct (decompose_prod_assum [] t0). *)
+(*   rewrite <- H. *)
+(*   destruct (decompose_app t1) as [fn arg] eqn:?. *)
+(*   rewrite (decompose_app_subst _ _ _ fn arg); auto. simpl. *)
+(*   destruct (chop _ arg) eqn:Heqchop. eapply chop_map in Heqchop. *)
+(*   rewrite Heqchop. clear Heqchop. *)
+(*   unfold on_snd. simpl. f_equal. *)
+(*   rewrite subst_it_mkProd_or_LetIn, !subst_mkApps, map_app; simpl. *)
+(*   rewrite !subst_mkApps, !map_app, subst_context_length. *)
+(*   rewrite permute_subst by lia. repeat f_equal. *)
+(*   now rewrite to_extended_list_subst, <- to_extended_list_map_subst. *)
+(*   simpl. reflexivity. *)
+(*   specialize (H _ eq_refl). rewrite H. clear H. *)
+(*   rewrite map_option_out_map_option_map. *)
+(*   destruct (map_option_out (build_branches_type _ _ _ _ _ _)). *)
+(*   intros [= -> -> -> <-]. reflexivity. congruence. *)
+(* Qed. *)
+Admitted.
+
+Hint Unfold subst1 : subst.
+Hint Rewrite subst_mkApps distr_subst: subst.
+
+Lemma subs_nth_error `{checker_flags} Σ Γ s Δ decl n t :
+  subs Σ Γ s Δ ->
+  nth_error Δ n = Some decl ->
+  nth_error s n = Some t ->
+  match decl_body decl return Type with
+  | Some t' => False
+  | None =>
+    let ty := substl (skipn (S n) s) (decl_type decl) in
+    Σ ;;; Γ |- t : ty
+  end.
+Proof.
+  induction 1 in n |- *; simpl; auto; destruct n; simpl; try congruence.
+  - intros [= <-]. intros [= ->].
+    simpl. exact t1.
+  - apply IHX.
+Qed.
+
+Lemma red1_tApp_mkApps_l Σ Γ M1 N1 M2 :
+  red1 Σ Γ M1 N1 -> red1 Σ Γ (tApp M1 M2) (mkApps N1 M2).
+Proof. constructor. auto. Qed.
+Lemma mkApp_mkApps f a l : mkApp (mkApps f l) a = mkApps f (l ++ [a]).
+Proof.
+  destruct l. simpl. reflexivity.
+  rewrite <- mkApp_nested. reflexivity.
+Qed.
+
+Lemma red1_tApp_mkApp Σ Γ M1 N1 M2 :
+  red1 Σ Γ M1 N1 -> red1 Σ Γ (tApp M1 [M2]) (mkApp N1 M2).
+Proof.
+  intros.
+  change (mkApp N1 M2) with (mkApps N1 [M2]).
+  apply app_red_l. auto.
+Qed.
+
+Lemma nth_error_app_left {A} (l l' : list A) n t : nth_error l n = Some t -> nth_error (l ++ l') n = Some t.
+Proof. induction l in n |- *; destruct n; simpl; try congruence. auto. Qed.
+
+Lemma mkApp_tApp f u : isApp f = false -> mkApp f u = tApp f [u].
+Proof. intros. destruct f; (discriminate || reflexivity). Qed.
+
+Lemma red1_mkApp Σ Γ M1 N1 M2 :
+  Ast.wf M1 ->
+  red1 Σ Γ M1 N1 -> red1 Σ Γ (mkApp M1 M2) (mkApp N1 M2).
+Proof.
+  intros wfM1 H.
+  destruct (isApp M1) eqn:Heq.
+  destruct M1; try discriminate. simpl.
+  revert wfM1. inv H. simpl. intros.
+  rewrite mkApp_mkApps. constructor.
+
+  intros. inv wfM1. simpl.
+  econstructor; eauto.
+  clear -H1.
+  unfold is_constructor in *.
+  destruct (nth_error l narg) eqn:Heq.
+  eapply nth_error_app_left in Heq. now rewrite Heq. discriminate.
+
+  intros. rewrite mkApp_mkApps. now constructor.
+
+  intros. simpl.
+  constructor. clear -H0. induction H0; constructor; auto.
+
+  rewrite mkApp_tApp; auto.
+  now apply red1_tApp_mkApp.
+Qed.
+
+Lemma red1_mkApps_l Σ Γ M1 N1 M2 :
+  Ast.wf M1 -> Forall Ast.wf M2 ->
+  red1 Σ Γ M1 N1 -> red1 Σ Γ (mkApps M1 M2) (mkApps N1 M2).
+Proof.
+  induction M2 in M1, N1 |- *. simpl; auto.
+  intros. specialize (IHM2 (mkApp M1 a) (mkApp N1 a)).
+  inv H0.
+  forward IHM2. apply wf_mkApp; auto.
+  forward IHM2. auto.
+  rewrite <- !mkApps_mkApp; auto.
+  apply IHM2.
+  apply red1_mkApp; auto.
+Qed.
+
+Lemma OnOne2_app {A} (P : A -> A -> Type) l tl tl' : OnOne2 P tl tl' -> OnOne2 P (l ++ tl) (l ++ tl').
+Proof. induction l; simpl; try constructor; auto. Qed.
+
+Lemma red1_mkApps_r Σ Γ M1 M2 N2 :
+  Ast.wf M1 -> Forall Ast.wf M2 ->
+  OnOne2 (red1 Σ Γ) M2 N2 -> red1 Σ Γ (mkApps M1 M2) (mkApps M1 N2).
+Proof.
+  intros. induction H1 in M1, H, H0 |- *.
+  inv H0.
+  destruct (isApp M1) eqn:Heq. destruct M1; try discriminate.
+  simpl. constructor. apply OnOne2_app. constructor. auto.
+  rewrite mkApps_tApp; try congruence.
+  rewrite mkApps_tApp; try congruence.
+  constructor. constructor. auto.
+  inv H0.
+  specialize (IHOnOne2 (mkApp M1 hd)). forward IHOnOne2.
+  apply wf_mkApp; auto. forward IHOnOne2; auto.
+  now rewrite !mkApps_mkApp in IHOnOne2.
+Qed.
+
+Lemma substitution_red1 `{CF:checker_flags} Σ Γ Γ' Γ'' s M N :
+  wf Σ -> Forall Ast.wf s -> subs Σ Γ s Γ' -> wf_local Σ Γ -> Ast.wf M ->
+  red1 (fst Σ) (Γ ,,, Γ' ,,, Γ'') M N ->
+  red1 (fst Σ) (Γ ,,, subst_context s 0 Γ'') (subst s #|Γ''| M) (subst s #|Γ''| N).
+Proof.
+  intros wfΣ wfs Hs wfΓ wfM H.
+  remember (Γ ,,, Γ' ,,, Γ'') as Γ0. revert Γ Γ' Γ'' HeqΓ0 wfΓ Hs.
+  induction H using red1_ind_all in |- *; intros Γ0 Γ' Γ'' HeqΓ0 wfΓ Hs; try subst Γ; simpl;
+    autorewrite with subst;
+    try solve [  econstructor; try inv wfM; eauto ].
+
+  - unfold subst1. rewrite distr_subst; auto. constructor.
+  - unfold subst1. rewrite distr_subst; auto. constructor.
+
+  - pose proof (subst_length _ _ _ _ Hs).
+    elim (leb_spec_Set); intros Hn.
+    + destruct (nth_error s) eqn:Heq.
+      ++ pose proof (nth_error_Some_length Heq).
+         rewrite nth_error_app_ge in H by lia.
+         rewrite nth_error_app_lt in H by lia.
+         destruct nth_error eqn:HΓ'.
+         eapply subs_nth_error in Heq; eauto.
+         simpl in H. destruct decl_body; try contradiction.
+         discriminate. discriminate.
+      ++ apply nth_error_None in Heq.
+         assert(S i = #|s| + (S (i - #|s|))) by lia.
+         rewrite H1. rewrite simpl_subst; try lia.
+         econstructor.
+         rewrite nth_error_app_ge in H by lia.
+         rewrite nth_error_app_ge in H by lia.
+         rewrite nth_error_app_ge. 2:(autorewrite with wf; lia).
+         rewrite <- H. f_equal. f_equal. autorewrite with wf. lia.
+         rewrite !nth_error_app_ge in H by lia.
+         destruct nth_error eqn:Hi.
+         eapply nth_error_All_local_env in wfΓ. red in wfΓ.
+         rewrite Hi in wfΓ. simpl in H.
+         destruct c; simpl in H; try discriminate.
+         injection H. intros ->. red in wfΓ. cbn in *. apply typing_wf in wfΓ. intuition eauto. eauto.
+         eapply typing_wf_local in wfΓ; eauto.
+         apply nth_error_Some_length in Hi. lia. discriminate.
+    + rewrite nth_error_app_lt in H by lia.
+      pose (commut_lift_subst_rec body s (S i) (#|Γ''| - S i) 0).
+      assert(eq:(S i + (#|Γ''| - S i)) = #|Γ''|) by lia.
+      rewrite eq in e. rewrite <- e by lia.
+      constructor.
+      rewrite nth_error_app_lt by (autorewrite with wf; lia).
+      rewrite nth_error_subst_context.
+      unfold subst_decl; now rewrite option_map_decl_body_map_decl, H, Nat.add_0_r.
+
+  - rewrite subst_iota_red.
+    constructor.
+
+  - inv wfM. rewrite mkApps_tApp; simpl; auto with wf.
+    rewrite mkApps_tApp; simpl; auto with wf.
+    eapply red_fix. erewrite subst_unfold_fix; eauto.
+    now apply subst_is_constructor.
+    inv H3.
+    unfold unfold_fix in H.
+    destruct nth_error eqn:Heq.
+    injection H. intros <- <-.
+    eapply nth_error_forall in H5; eauto.
+    destruct d as [na b ty]; simpl in *.
+    destruct H5 as [_ [_ Hty]].
+    destruct ty; try discriminate.
+    discriminate.
+
+  - pose proof (subst_declared_constant _ _ _ s #|Γ''| wfΣ H).
+    pose proof (declared_decl_closed _ _ _ wfΣ H). simpl in X.
+    red in X. destruct decl; try discriminate. simpl in *. subst cst_body.
+    rewrite andb_true_iff in X. intuition.
+    unfold map_constant_body in H1. simpl in *.
+    pose proof (closedn_subst_instance_constr #|Γ''| body u).
+    eapply closed_upwards in H2. rewrite <- H4 in H2.
+    eapply subst_closedn in H2. rewrite H2.
+    econstructor. eauto. eauto.
+    wf. lia.
+
+  - inv wfM.
+    simpl. constructor.
+    now rewrite nth_error_map, H.
+
+  - constructor.
+    inv wfM.
+    specialize (IHred1 H1 Γ0 Γ' (Γ'' ,, vass na N) eq_refl).
+    rewrite subst_context_snoc, Nat.add_0_r in IHred1. now apply IHred1.
+
+  - constructor.
+    inv wfM.
+    specialize (IHred1 H2 Γ0 Γ' (Γ'' ,, _) eq_refl).
+    rewrite subst_context_snoc, Nat.add_0_r in IHred1. now apply IHred1.
+
+  - inv wfM. constructor.
+    induction H; constructor; auto.
+    intuition; eauto.
+    inv H2. specialize (H3 H4 _ _ _ eq_refl).
+    destruct hd, hd'; simpl in *. now eapply H3.
+    eapply IHOnOne2. inv H2; eauto.
+
+  - inv wfM.
+    specialize (IHred1 H2 _ _ _ eq_refl).
+    specialize (IHred1 wfΓ Hs).
+    apply red1_mkApps_l. apply wf_subst; auto.
+    apply Forall_map; eapply Forall_impl. eauto.
+    intros. now apply wf_subst.
+    apply IHred1.
+
+  - inv wfM.
+    apply red1_mkApps_r; auto with wf.
+    apply Forall_map. eapply Forall_impl; eauto. simpl; eauto with wf.
+    clear -H H2 H3 wfΓ Hs.
+    induction H; constructor; auto.
+    inv H3. intuition.
+    eapply H4; eauto.
+    apply IHOnOne2. inv H3. eauto.
+
+  - inv wfM.
+    constructor. specialize (IHred1 H1 _ _ (Γ'' ,, vass na M1) eq_refl).
+    rewrite subst_context_snoc, Nat.add_0_r in IHred1.
+    now eapply IHred1.
+
+  - inv wfM.
+    constructor.
+    induction H; constructor; auto.
+    inv H0. intuition. eapply H3; eauto.
+    apply IHOnOne2. now inv H0.
+Qed.
+
+Conjecture eq_universe_refl : forall `{checker_flags} φ u, eq_universe φ u u = true.
+Conjecture eq_universe_instance_refl : forall `{checker_flags} φ u, eq_universe_instance φ u u = true.
+Conjecture eq_universe_leq_universe : forall `{checker_flags} φ x y,
+    eq_universe φ x y = true ->
+    leq_universe φ x y = true.
+
+Lemma eq_string_refl x : eq_string x x = true.
+Proof. unfold eq_string. destruct string_dec; congruence. Qed.
+
+Lemma eq_ind_refl i : eq_ind i i = true.
+Proof.
+  destruct i as [mind k].
+  unfold eq_ind. now rewrite eq_string_refl, Nat.eqb_refl.
+Qed.
+
+Lemma eq_projection_refl i : eq_projection i i = true.
+Proof.
+  destruct i as [[mind k] p].
+  unfold eq_projection.
+  now rewrite eq_ind_refl, !Nat.eqb_refl.
+Qed.
+
+Lemma eq_term_refl `{checker_flags} φ t : eq_term φ t t = true.
+Proof.
+  induction t using term_forall_list_ind; simpl; try reflexivity; try discriminate;
+    try (merge_Forall; close_Forall; intuition auto);
+    try (rewrite ?IHt1, ?IHt2, ?IHt3; reflexivity).
+
+  - apply Nat.eqb_refl.
+  - apply eq_string_refl.
+  - apply Nat.eqb_refl.
+  - unfold eq_evar. rewrite Nat.eqb_refl.
+    simpl. induction H0; simpl; auto. now rewrite H0, IHForall.
+  - apply eq_universe_refl.
+  - eapply (Forall_forallb _ _ (fun x => eq_term φ x x)) in H0.
+    rewrite IHt. induction l; simpl; auto.
+    simpl in H0. rewrite andb_true_iff in H0. intuition.
+    auto.
+  - unfold eq_constant. rewrite eq_string_refl.
+    apply eq_universe_instance_refl.
+  - rewrite eq_ind_refl. apply eq_universe_instance_refl.
+  - rewrite eq_ind_refl. rewrite Nat.eqb_refl. apply eq_universe_instance_refl.
+  - destruct p. simpl.
+    rewrite eq_ind_refl, Nat.eqb_refl, IHt1, IHt2.
+    simpl. induction l.
+    reflexivity.
+    simpl. destruct a. inv H0. simpl in H1. rewrite H1.
+    rewrite IHl; auto.
+  - now rewrite eq_projection_refl, IHt.
+  - rewrite Nat.eqb_refl.
+    induction m. reflexivity.
+    inv H0. intuition.
+    simpl. rewrite H0, H3. simpl. apply H1.
+  - rewrite Nat.eqb_refl.
+    induction m. reflexivity.
+    inv H0. intuition.
+    simpl. rewrite H0, H3. simpl. apply H1.
+Qed.
+
+Lemma eq_term_leq_term `{checker_flags} φ t u : eq_term φ t u = true -> leq_term φ t u = true.
+Proof.
+  induction t in u |- * using term_forall_list_ind; simpl; intros; auto; try reflexivity; try discriminate;
+    try (merge_Forall; close_Forall; intuition auto);
+    try (rewrite ?IHt1, ?IHt2, ?IHt3; reflexivity).
+
+  - destruct u; try discriminate. now apply eq_universe_leq_universe.
+  - destruct u; try discriminate.
+    rewrite andb_true_iff in *. intuition.
+  - destruct u; try discriminate.
+    rewrite andb_true_iff in *. intuition.
+  - destruct u; try discriminate.
+    rewrite andb_true_iff in *. intuition.
+Qed.
+
+Lemma eq_term_App `{checker_flags} φ f f' :
+  eq_term φ f f' = true ->
+  isApp f = isApp f'.
+Proof.
+  destruct f, f'; simpl; try congruence.
+  destruct p. auto.
+Qed.
+
+Lemma forallb2_app {A} (p : A -> A -> bool) l l' q q' :
+  forallb2 p l l' && forallb2 p q q' = true -> forallb2 p (l ++ q) (l' ++ q') = true.
+Proof.
+  induction l in l' |- *; destruct l'; simpl; try congruence.
+  intros.
+  rewrite !andb_true_iff in *.
+  rewrite IHl; intuition auto. now rewrite H2, H1.
+Qed.
+
+Lemma eq_term_mkApps `{checker_flags} φ f l f' l' :
+  eq_term φ f f' = true ->
+  forallb2 (eq_term φ) l l' = true ->
+  eq_term φ (mkApps f l) (mkApps f' l') = true.
+Proof.
+  induction l in f, f' |- *; destruct l'; try (simpl; congruence).
+  intros.
+  destruct (isApp f) eqn:Hf.
+  pose (eq_term_App _ _ _ H0). rewrite Hf in e.
+  destruct f; try discriminate.
+  destruct f'; try discriminate.
+  simpl in *.
+  rewrite andb_true_iff in *. intuition.
+  rewrite forallb2_app; auto.
+  simpl. now rewrite H3, H0, H4.
+
+  rewrite !mkApps_tApp; auto. simpl. rewrite H0.
+  apply H1.
+  pose (eq_term_App _ _ _ H0). all:congruence.
+Qed.
+
+Lemma leq_term_mkApps `{checker_flags} φ f l f' l' :
+  eq_term φ f f' = true ->
+  forallb2 (eq_term φ) l l' = true ->
+  leq_term φ (mkApps f l) (mkApps f' l') = true.
+Proof.
+  induction l in f, f' |- *; destruct l'; try (simpl; congruence).
+  intros. simpl. apply eq_term_leq_term. auto.
+  intros.
+  destruct (isApp f) eqn:Hf.
+  pose (eq_term_App _ _ _ H0). rewrite Hf in e.
+  destruct f; try discriminate.
+  destruct f'; try discriminate.
+  simpl in *.
+  rewrite andb_true_iff in *. intuition.
+  rewrite forallb2_app; auto.
+  simpl. now rewrite H3, H0, H4.
+
+  rewrite !mkApps_tApp; auto. simpl. rewrite H0.
+  apply H1.
+  pose (eq_term_App _ _ _ H0). all:congruence.
+Qed.
+
+Lemma subst_eq_term `{checker_flags} ϕ n k T U :
+  eq_term ϕ T U = true ->
+  eq_term ϕ (subst n k T) (subst n k U) = true.
+Proof.
+  intros Hleq.
+  induction T in n, k, U, Hleq |- * using term_forall_list_ind; intros;
+    destruct U; try discriminate;
+  try solve [simpl; auto]; try
+                             (destruct (mkApps_trans_wf _ _ H0) as [U' [V' ->]]; reflexivity);
+  simpl in *; revert Hleq; try rewrite !andb_true_iff in *; intuition auto;
+    try (merge_Forall; close_Forall; intuition auto).
+
+  - intros.
+    apply Nat.eqb_eq in Hleq. subst.
+    destruct (leb_spec_Set k n1).
+    destruct nth_error eqn:Heq. apply eq_term_refl.
+    apply eq_term_refl.
+    apply eq_term_refl.
+
+  - apply eq_term_mkApps. eauto. eauto.
+    merge_Forall. eapply Forall2_impl; eauto.
+    simpl; intros; intuition auto.
+
+  - destruct p. destruct Nat.leb. discriminate. discriminate.
+  - destruct p. discriminate.
+  - destruct p, p0. rewrite !andb_true_iff in *. intuition auto.
+    red in H0. merge_Forall. close_Forall. intuition auto. destruct y. simpl. auto.
+  - rewrite !andb_true_iff in *.
+    destruct x, y; simpl in *; intuition auto.
+    assert (#|m| = #|m0|). clear -H2. induction H2; simpl; auto. rewrite H4. auto.
+  - rewrite !andb_true_iff in *.
+    destruct x, y; simpl in *; intuition auto.
+    assert (#|m| = #|m0|). clear -H2. induction H2; simpl; auto. rewrite H4. auto.
+Qed.
+
+Lemma forallb2_forallb2 {A} (f : A -> A -> bool) g l l' :
+  (forall x y, f x y = true -> f (g x) (g y) = true) ->
+  forallb2 f l l' = true -> forallb2 f (map g l) (map g l') = true.
+Proof.
+  induction l in l' |- *; destruct l'; auto.
+  simpl; intros.
+  rewrite andb_true_iff in *. intuition.
+Qed.
+
+Lemma subst_leq_term `{checker_flags} ϕ n k T U :
+  leq_term ϕ T U = true ->
+  leq_term ϕ (subst n k T) (subst n k U) = true.
+Proof.
+  intros Hleq.
+  induction T in n, k, U, Hleq |- * using term_forall_list_ind; intros;
+    destruct U; try discriminate;
+  try solve [simpl; auto]; try
+                             (destruct (mkApps_trans_wf _ _ H0) as [U' [V' ->]]; reflexivity);
+  simpl in *; revert Hleq; try destruct p, p0; try rewrite !andb_true_iff in *;
+    intuition auto using subst_eq_term;
+    try (merge_Forall; close_Forall; intuition eauto using subst_eq_term).
+
+  - apply Nat.eqb_eq in Hleq. subst.
+    destruct Nat.leb; simpl. destruct nth_error.
+    eapply eq_term_leq_term. apply eq_term_refl. simpl.
+    apply Nat.eqb_refl. apply Nat.eqb_refl.
+  - apply leq_term_mkApps.
+    now apply subst_eq_term.
+    apply forallb2_forallb2; auto using subst_eq_term.
+  - destruct p. discriminate.
+  - destruct p; discriminate.
+  - destruct y. simpl. auto using subst_eq_term.
+  - rewrite !andb_true_iff in *.
+    destruct x, y; simpl in *; intuition auto using subst_eq_term.
+    assert (#|m| = #|m0|). clear -H2. induction H2; simpl; auto. rewrite H4.
+    auto using subst_eq_term.
+  - rewrite !andb_true_iff in *.
+    destruct x, y; simpl in *; intuition auto using subst_eq_term.
+    assert (#|m| = #|m0|). clear -H2. induction H2; simpl; auto. rewrite H4.
+    auto using subst_eq_term.
+Qed.
+
+Lemma subs_wf `{checker_flags} Σ Γ s Δ : wf Σ -> subs Σ Γ s Δ -> Forall Ast.wf s.
+Proof.
+  induction 2; constructor.
+  apply typing_wf in t0; intuition auto with wf.
+  eapply typing_wf_local in t0; eauto.
+  auto.
+Qed.
+
+
+Lemma wf_red1_wf `{checker_flags} Σ Γ M N : wf Σ -> wf_local Σ Γ -> Ast.wf M -> red1 (fst Σ) Γ M N -> Ast.wf N.
+Proof.
+  intros wfΣ wfΓ wfM Hr.
+  apply wf_red1 in Hr; eauto.
+  apply typing_wf_sigma; auto.
+  apply typing_all_wf_decl in wfΓ; eauto.
+  eapply Forall_impl; eauto.
+  intros x Hx. red in Hx. destruct decl_body; intuition.
+Qed.
+
+Lemma substitution_cumul `{CF:checker_flags} Σ Γ Γ' Γ'' s M N :
+  wf Σ -> wf_local Σ (Γ ,,, Γ' ,,, Γ'') -> subs Σ Γ s Γ' -> Ast.wf M -> Ast.wf N ->
+  Σ ;;; Γ ,,, Γ' ,,, Γ'' |- M <= N ->
+  Σ ;;; Γ ,,, subst_context s 0 Γ'' |- subst s #|Γ''| M <= subst s #|Γ''| N.
+Proof.
+  intros wfΣ wfΓ Hs wfM wfN. induction 1.
+  constructor.
+  - now apply subst_leq_term.
+  - pose proof H.
+    apply wf_red1_wf in H1; eauto.
+    eapply substitution_red1 in H. 4:eauto. all:auto.
+    econstructor 2; eauto.
+    eauto using subs_wf.
+    eauto with wf.
+  - pose proof H0.
+    apply wf_red1_wf in H1; eauto.
+    eapply substitution_red1 in H0. 4:eauto.
+    all:eauto using subs_wf with wf.
+    now econstructor 3.
+Qed.
+
+Theorem substitution `{checker_flags} Σ Γ Γ' s Δ (t : term) T :
+  wf Σ -> wf_local Σ Γ ->
+  subs Σ Γ s Γ' ->
+  Σ ;;; Γ ,,, Γ' ,,, Δ |- t : T ->
+  Σ ;;; Γ ,,, map_context (substl s) Δ |- substl s t : substl s T.
+Proof.
+  intros HΣ HΓ * Ht Hu.
+Admitted.
+
+Lemma substitution0 `{checker_flags} Σ Γ n u U (t : term) :
+  wf Σ -> wf_local Σ Γ ->
+  `(Σ ;;; Γ ,, vass n U |- t : T -> Σ ;;; Γ |- u : U ->
+    Σ ;;; Γ |- t {0 := u} : T {0 := u}).
+Proof.
+  intros HΣ HΓ * Ht Hu.
+Admitted.
