template-coq/theories/WeakeningEnv.v
@@ -1,0 +1,263 @@
+(* Distributed under the terms of the MIT license.   *)
+
+From Coq Require Import Bool String List Program BinPos Compare_dec Omega Lia.
+From Template Require Import config utils Ast AstUtils Induction utils LiftSubst Typing.
+
+(** * Weakening lemmas w.r.t. the global environment *)
+
+
+Set Asymmetric Patterns.
+
+Generalizable Variables Σ Γ t T.
+
+Definition extends (Σ Σ' : global_context) :=
+  exists Σ'', Σ' = (Σ'' ++ fst Σ, snd Σ)%list.
+
+Lemma lookup_env_Some_fresh `{checker_flags} Σ φ c decl :
+  wf (Σ, φ) -> lookup_env Σ c = Some decl ->
+  ~ (fresh_global c Σ).
+Proof. unfold wf. unfold on_global_env; simpl.
+  induction 1; simpl. congruence.
+  destruct ident_eq eqn:Heq. intros [= ->].
+  rewrite <- (reflect_iff _ _ (ident_eq_spec _ _)) in Heq.
+  intro. inv H0. congruence.
+  intros Hl; specialize (IHX Hl).
+  intro. inv H0. contradiction.
+Qed.
+
+Lemma extends_lookup `{checker_flags} Σ Σ' c decl :
+  wf Σ' -> extends Σ Σ' ->
+  lookup_env (fst Σ) c = Some decl -> lookup_env (fst Σ') c = Some decl.
+Proof.
+  intros wfΣ' [Σ'' ->]. simpl.
+  induction Σ'' in wfΣ', c, decl |- *. simpl. auto.
+  specialize (IHΣ'' c decl). forward IHΣ''.
+  inv wfΣ'. simpl in X0. apply X.
+  intros HΣ. specialize (IHΣ'' HΣ).
+  inv wfΣ'. simpl in *.
+  destruct (ident_eq c (global_decl_ident a)) eqn:Heq'.
+  eapply lookup_env_Some_fresh in IHΣ''; eauto.
+  rewrite <- (reflect_iff _ _ (ident_eq_spec _ _)) in Heq'.
+  rewrite <- Heq' in H0. contradiction.
+  auto.
+Qed.
+Hint Resolve extends_lookup : extends.
+
+Lemma extends_wf_local:
+  forall (H : checker_flags) (Σ : global_context) (Γ : context),
+    wf_local Σ Γ ->
+    All_local_env
+      (fun (Σ0 : global_context) (Γ0 : context) (t T : term) =>
+         forall Σ' : global_context, wf Σ' -> extends Σ0 Σ' -> Σ';;; Γ0 |- t : T) Σ Γ ->
+    forall Σ' : global_context, wf Σ' -> extends Σ Σ' -> wf_local Σ' Γ.
+Proof.
+  intros H Σ Γ X X0 Σ' H0.
+  induction X; inv X0; try econstructor; auto.
+Qed.
+Hint Resolve extends_wf_local : extends.
+
+Lemma weakening_env_red1 `{CF:checker_flags} Σ Σ' Γ M N :
+  wf Σ' -> extends Σ Σ' ->
+  red1 (fst Σ) Γ M N ->
+  red1 (fst Σ') Γ M N.
+Proof.
+  induction 3 using red1_ind_all; try econstructor; eauto.
+  eapply extends_lookup in H0; eauto.
+
+  induction H0; constructor; intuition eauto.
+  induction H0; constructor; intuition eauto.
+  induction H0; constructor; intuition eauto.
+Qed.
+
+Lemma weakening_env_cumul `{CF:checker_flags} Σ Σ' Γ M N :
+  wf Σ' -> extends Σ Σ' ->
+  cumul Σ Γ M N -> cumul Σ' Γ M N.
+Proof.
+  intros wfΣ [Σ'' ->].
+  induction 1; simpl.
+
+  econstructor; eauto.
+
+  econstructor 2; eauto. eapply weakening_env_red1; eauto. exists Σ''; eauto.
+  econstructor 3; eauto. eapply weakening_env_red1; eauto. exists Σ''; eauto.
+Qed.
+
+Lemma weakening_env_consistent_universe_context_instance:
+  forall (Σ : global_context) (u : list Level.t) univs,
+    consistent_universe_context_instance Σ univs u ->
+    forall Σ' : global_context,
+      extends Σ Σ' -> consistent_universe_context_instance Σ' univs u.
+Proof.
+  intros Σ u univs H1 Σ' H2. destruct univs; simpl in *; eauto.
+  destruct UContext.dest. destruct H2 as [Σ'' ->]. simpl. auto.
+Qed.
+Hint Resolve weakening_env_consistent_universe_context_instance : extends.
+
+Lemma weakening_env_declared_constant:
+  forall (H : checker_flags) (Σ : global_context) (cst : ident) (decl : constant_body),
+    declared_constant (fst Σ) cst decl ->
+    forall Σ' : global_context, wf Σ' -> extends Σ Σ' -> declared_constant (fst Σ') cst decl.
+Proof.
+  intros H Σ cst decl H0 Σ' X2 H2.
+  eapply extends_lookup; eauto.
+Qed.
+Hint Resolve weakening_env_declared_constant : extends.
+
+Lemma weakening_env_declared_minductive:
+  forall (H : checker_flags) (Σ : global_context) ind decl,
+    declared_minductive (fst Σ) ind decl ->
+    forall Σ' : global_context, wf Σ' -> extends Σ Σ' -> declared_minductive (fst Σ') ind decl.
+Proof.
+  intros H Σ cst decl H0 Σ' X2 H2.
+  eapply extends_lookup; eauto.
+Qed.
+Hint Resolve weakening_env_declared_minductive : extends.
+
+Lemma weakening_env_declared_inductive:
+  forall (H : checker_flags) (Σ : global_context) ind mdecl decl,
+    declared_inductive (fst Σ) ind mdecl decl ->
+    forall Σ' : global_context, wf Σ' -> extends Σ Σ' -> declared_inductive (fst Σ') ind mdecl decl.
+Proof.
+  intros H Σ cst decl H0 [Hmdecl Hidecl] Σ' X2 H2. split; eauto with extends.
+Qed.
+Hint Resolve weakening_env_declared_inductive : extends.
+
+Lemma weakening_env_declared_constructor :
+  forall (H : checker_flags) (Σ : global_context) ind mdecl idecl decl,
+    declared_constructor (fst Σ) ind mdecl idecl decl ->
+    forall Σ' : global_context, wf Σ' -> extends Σ Σ' ->
+    declared_constructor (fst Σ') ind mdecl idecl decl.
+Proof.
+  intros H Σ cst mdecl idecl cdecl [Hidecl Hcdecl] Σ' X2 H2.
+  split; eauto with extends.
+Qed.
+Hint Resolve weakening_env_declared_constructor : extends.
+
+Lemma weakening_env_declared_projection :
+  forall (H : checker_flags) (Σ : global_context) ind mdecl idecl decl,
+    declared_projection (fst Σ) ind mdecl idecl decl ->
+    forall Σ' : global_context, wf Σ' -> extends Σ Σ' ->
+    declared_projection (fst Σ') ind mdecl idecl decl.
+Proof.
+  intros H Σ cst mdecl idecl cdecl [Hidecl Hcdecl] Σ' X2 H2.
+  split; eauto with extends.
+Qed.
+Hint Resolve weakening_env_declared_projection : extends.
+
+Lemma weakening_All_local_env_impl `{checker_flags}
+      (P Q : global_context -> context -> term -> term -> Type) Σ Σ' l :
+  All_local_env P Σ l ->
+  (forall Γ t T, P Σ Γ t T -> Q Σ' Γ t T) ->
+  All_local_env Q Σ' l.
+Proof.
+  induction 1; intros; simpl; econstructor; eauto. Qed.
+
+Lemma weakening_env `{checker_flags} :
+  env_prop (fun Σ Γ t T =>
+              forall Σ', wf Σ' -> extends Σ Σ' -> Σ' ;;; Γ |- t : T).
+Proof.
+  apply typing_ind_env; intros; try solve [econstructor; eauto 2 with extends].
+
+  - econstructor; eauto.
+    clear H0 H1 X X0. induction X1 in wfΓ |- *; econstructor; eauto.
+    eapply weakening_env_cumul in cumul; eauto.
+  - econstructor; eauto 2 with extends.
+    destruct H6 as [Σ'' ->]. simpl; auto.
+    close_Forall. intros; intuition eauto with extends.
+  - econstructor; eauto with extends.
+    eapply weakening_All_local_env_impl. eapply X.
+    clear -X1 H1. simpl; intros. intuition eauto with extends.
+    eapply All_impl; eauto; simpl; intuition eauto with extends.
+  - econstructor; eauto with extends.
+    eapply weakening_All_local_env_impl. eapply X.
+    clear -X1 H1. simpl; intros. intuition eauto with extends.
+    eapply All_impl; eauto; simpl; intuition eauto with extends.
+  - eapply weakening_env_cumul in H0; eauto. econstructor; eauto.
+Qed.
+
+
+Definition weaken_env_prop `{checker_flags}
+           (P : global_context -> context -> option term -> term -> Type) :=
+  forall Σ Σ', wf Σ' -> extends Σ Σ' -> forall Γ t T, P Σ Γ t T -> P Σ' Γ t T.
+
+Lemma weakening_on_global_decl `{checker_flags} P Σ Σ' decl :
+  weaken_env_prop P ->
+  wf Σ' -> extends Σ Σ' ->
+  on_global_decl P Σ decl ->
+  on_global_decl P Σ' decl.
+Proof.
+  unfold weaken_env_prop.
+  intros HPΣ wfΣ' Hext Hdecl.
+  destruct decl. destruct c. destruct cst_body. simpl in *.
+  red in Hdecl |- *. simpl in *.
+  eapply HPΣ; eauto.
+  eapply HPΣ; eauto.
+  simpl in *.
+  do 2 red in Hdecl. eapply Alli_impl; eauto.
+  intros.
+  destruct X. constructor.
+  unfold on_type in *; eauto.
+  unfold on_constructors in *. eapply All_impl; eauto.
+  intros [[id t] ar]. unfold on_constructor, on_type in *; eauto.
+  destruct decompose_prod_assum. intuition.
+  eapply All_impl; eauto. intros [id trm].
+  unfold on_projection, on_type; eauto.
+Qed.
+
+Lemma weakening_env_lookup_on_global_env `{checker_flags} P Σ Σ' c decl :
+  weaken_env_prop P ->
+  wf Σ' -> extends Σ Σ' -> on_global_env P Σ ->
+  lookup_env (fst Σ) c = Some decl ->
+  on_global_decl P Σ' decl.
+Proof.
+  intros HP wfΣ Hext HΣ. destruct Σ as [Σ graph].
+  red in HΣ. simpl in *.
+  induction HΣ; simpl. congruence.
+  destruct ident_eq. intros [= ->].
+  eapply weakening_on_global_decl. eauto. eauto. 2:{ eapply o. }
+  destruct Hext. simpl in *. rewrite H0.
+  exists ((x ++ [decl])%list). simpl.
+  now rewrite <- app_assoc.
+
+  apply IHHΣ.
+  destruct Hext as [Σ'' ->]. simpl. red.
+  exists (Σ'' ++ [d])%list. simpl.
+  now rewrite <- app_assoc.
+Qed.
+
+Lemma weaken_lookup_on_global_env `{checker_flags} P Σ c decl :
+  weaken_env_prop P ->
+  wf Σ -> on_global_env P Σ ->
+  lookup_env (fst Σ) c = Some decl ->
+  on_global_decl P Σ decl.
+Proof.
+  intros. eapply weakening_env_lookup_on_global_env; eauto.
+  exists []; simpl; destruct Σ; eauto.
+Qed.
+
+Lemma declared_minductive_inv `{checker_flags} Σ P ind mdecl :
+  weaken_env_prop (lift_typing P) ->
+  wf Σ -> Forall_decls_typing P Σ ->
+  declared_minductive (fst Σ) ind mdecl ->
+  on_inductive (lift_typing P) Σ ind
+               (polymorphic_instance (ind_universes mdecl))
+               (ind_npars mdecl) (ind_bodies mdecl).
+Proof.
+  intros.
+  eapply weaken_lookup_on_global_env in X1; eauto. apply X1.
+Qed.
+
+Lemma declared_inductive_inv `{checker_flags} Σ P ind mdecl idecl :
+  weaken_env_prop (lift_typing P) ->
+  wf Σ -> Forall_decls_typing P Σ ->
+  declared_inductive (fst Σ) ind mdecl idecl ->
+  on_ind_body (lift_typing P) Σ (inductive_mind ind)
+               (polymorphic_instance (ind_universes mdecl))
+               (ind_npars mdecl) (arities_context (ind_bodies mdecl)) (inductive_ind ind) idecl.
+Proof.
+  intros.
+  destruct H0 as [Hmdecl Hidecl].
+  eapply declared_minductive_inv in Hmdecl; eauto.
+  eapply nth_error_alli in Hidecl; eauto.
+  apply Hidecl.
+Qed.
